Utils.thy
@@ -1,18 +1,19 @@
 theory Utils imports Syntax begin
 
-free_constructors packet for PktIn | PktOut
-using packet.strong_exhaust apply auto done
-(* TODO: Are these warnings bad? Can I do something about them? *)
-(* TODO: Is it preferable to do this, or make every function matching on packets
-         a nominal_function? *)
-(* TODO: This works when done here but not when done in Syntax? *)
-
 fun slice :: "'a list \<Rightarrow> int \<Rightarrow> int \<Rightarrow> 'a list" where
   "slice xs n m = take (nat (m - n)) (drop (nat n) xs)"
 
 text\<open>Replaces [n:m) in the first input list with the second list.\<close>
 fun splice :: "'a list \<Rightarrow> int \<Rightarrow> int \<Rightarrow> 'a list \<Rightarrow> 'a list" where
   "splice xs n m ins = (slice xs 0 n) @ ins @ (slice xs m (int (length xs)))"
+
+section\<open>Nominal2 Lemmas\<close>
+
+lemma bind_eqvt[eqvt]: "p \<bullet> Option.bind x f = Option.bind (p \<bullet> x) (p \<bullet> f)"
+  by (cases x) auto
+
+lemma map_of_eqvt[eqvt]: "p \<bullet> map_of xs x = map_of (p \<bullet> xs) (p \<bullet> x)"
+  by (induct xs) auto
 
 section\<open>Headers\<close>
 
@@ -32,8 +33,6 @@ fun header_lookup :: "headers \<Rightarrow> instanc \<Rightarrow> bv option" whe
 fun header_update :: "headers \<Rightarrow> instanc \<Rightarrow> bv \<Rightarrow> headers" where
   "header_update (Headers h) i bs = Headers (h(i := Some bs))"
 
-thm map_update
-
 fun header_field_to_range_helper :: "int \<Rightarrow> field list \<Rightarrow> field_name \<Rightarrow> (int \<times> int)" where
   "header_field_to_range_helper acc ((Field fn fl)#fs) tgt = (if fn = tgt then (acc, acc + fl)
     else header_field_to_range_helper (acc + fl) fs tgt)" |
@@ -42,7 +41,7 @@ fun header_field_to_range_helper :: "int \<Rightarrow> field list \<Rightarrow> 
 fun header_field_to_range :: "header_type \<Rightarrow> field_name \<Rightarrow> (int \<times> int)" where
   "header_field_to_range (HeaderType _ fs) tgt = header_field_to_range_helper 0 fs tgt"
 
-section\<open>Heaps and Envs\<close>
+section\<open>Heaps\<close>
 
 instantiation heap :: pure begin
   definition permute_heap :: "perm \<Rightarrow> heap \<Rightarrow> heap"  where
@@ -57,20 +56,31 @@ fun heap_lookup_packet :: "heap \<Rightarrow> packet \<Rightarrow> bv" where
   "heap_lookup_packet (Heap In Out _) PktIn = In" |
   "heap_lookup_packet (Heap In Out _) PktOut = Out"
 
+lemma heap_lookup_packet_eqvt[eqvt]:
+  "p \<bullet> heap_lookup_packet h pkt = heap_lookup_packet (p \<bullet> h) (p \<bullet> pkt)"
+  by (simp add: permute_pure)
+
 fun heap_lookup_instance :: "heap \<Rightarrow> instanc \<Rightarrow> bv option" where
   "heap_lookup_instance (Heap _ _ (Headers insts)) i = insts i"
+
+lemma heap_lookup_instance_eqvt[eqvt]:
+  "p \<bullet> heap_lookup_instance h i = heap_lookup_instance (p \<bullet> h) (p \<bullet> i)"
+  by (simp add: permute_pure)
+
+section\<open>Environments\<close>
 
 (* Easier to work with than "var \<Rightarrow> heap" with Nominal2 because it has a finite support (I think) *)
 type_synonym env = "(var \<times> heap) list"
 
 fun env_lookup_packet :: "env \<Rightarrow> var \<Rightarrow> packet \<Rightarrow> bv option" where
   "env_lookup_packet \<epsilon> x p = map_option (\<lambda>h. heap_lookup_packet h p) (map_of \<epsilon> x)"
+
 fun env_lookup_instance :: "env \<Rightarrow> var \<Rightarrow> instanc \<Rightarrow> bv option" where
   "env_lookup_instance \<epsilon> x i = Option.bind (map_of \<epsilon> x) (\<lambda>h. heap_lookup_instance h i)"
+
 nominal_function env_lookup_sliceable :: "env \<Rightarrow> sliceable \<Rightarrow> bv option" where
   "env_lookup_sliceable \<epsilon> (SlPacket x p) = env_lookup_packet \<epsilon> x p" |
   "env_lookup_sliceable \<epsilon> (SlInstance x i) = env_lookup_instance \<epsilon> x i"
-  (*using [[simproc del: alpha_lst defined_all]]*)
   subgoal by (simp add: eqvt_def env_lookup_sliceable_graph_aux_def)
   subgoal by (erule env_lookup_sliceable_graph.induct) (auto)
   apply clarify
